Add a few more minor theorems about bytes

ELFSage/Util/ByteArray.lean
@@ -1,6 +1,6 @@
 --BigEndian
 
-def ByteArray.getUInt64BEfrom (bs : ByteArray) (offset : Nat) (h: bs.size - offset ≥ 8) : UInt64 := 
+def ByteArray.getUInt64BEfrom (bs : ByteArray) (offset : Nat) (h: bs.size - offset ≥ 8) : UInt64 :=
   (bs.get ⟨offset + 0, by omega⟩).toUInt64 <<< 0x38 |||
   (bs.get ⟨offset + 1, by omega⟩).toUInt64 <<< 0x30 |||
   (bs.get ⟨offset + 2, by omega⟩).toUInt64 <<< 0x28 |||
@@ -10,19 +10,44 @@ def ByteArray.getUInt64BEfrom (bs : ByteArray) (offset : Nat) (h: bs.size - offs
   (bs.get ⟨offset + 6, by omega⟩).toUInt64 <<< 0x08 |||
   (bs.get ⟨offset + 7, by omega⟩).toUInt64
 
-def ByteArray.getUInt32BEfrom (bs : ByteArray) (offset : Nat) (h: bs.size - offset ≥ 4) : UInt32 := 
+
+def UInt64.getBytesBEfrom (i : UInt64) : ByteArray :=
+  ⟨#[ (i >>> 0x38).toUInt8
+    , (i >>> 0x30).toUInt8
+    , (i >>> 0x28).toUInt8
+    , (i >>> 0x20).toUInt8
+    , (i >>> 0x18).toUInt8
+    , (i >>> 0x10).toUInt8
+    , (i >>> 0x8).toUInt8
+    , (i >>> 0x0).toUInt8
+    ]⟩
+
+def ByteArray.getUInt32BEfrom (bs : ByteArray) (offset : Nat) (h: bs.size - offset ≥ 4) : UInt32 :=
   (bs.get ⟨offset + 0, by omega⟩).toUInt32 <<< 0x18 |||
   (bs.get ⟨offset + 1, by omega⟩).toUInt32 <<< 0x10 |||
   (bs.get ⟨offset + 2, by omega⟩).toUInt32 <<< 0x08 |||
   (bs.get ⟨offset + 3, by omega⟩).toUInt32
 
-def ByteArray.getUInt16BEfrom (bs : ByteArray) (offset : Nat) (h: bs.size - offset ≥ 2) : UInt16 := 
+def UInt32.getBytesBEfrom (i : UInt32) : ByteArray :=
+  ⟨#[ (i >>> 0x18).toUInt8
+    , (i >>> 0x10).toUInt8
+    , (i >>> 0x8).toUInt8
+    , (i >>> 0x0).toUInt8
+    ]⟩
+
+def ByteArray.getUInt16BEfrom (bs : ByteArray) (offset : Nat) (h: bs.size - offset ≥ 2) : UInt16 :=
   (bs.get ⟨offset + 0, by omega⟩).toUInt16 <<< 0x08 |||
   (bs.get ⟨offset + 1, by omega⟩).toUInt16
 
+def UInt16.getBytesBEfrom (i : UInt16) : ByteArray :=
+  ⟨#[ (i >>> 0x8).toUInt8
+    , (i >>> 0x0).toUInt8
+    ]⟩
+
+
 --LittleEndian
 
-def ByteArray.getUInt64LEfrom (bs : ByteArray) (offset : Nat) (h: bs.size - offset ≥ 8) : UInt64 := 
+def ByteArray.getUInt64LEfrom (bs : ByteArray) (offset : Nat) (h: bs.size - offset ≥ 8) : UInt64 :=
   (bs.get ⟨offset + 7, by omega⟩).toUInt64 <<< 0x38 |||
   (bs.get ⟨offset + 6, by omega⟩).toUInt64 <<< 0x30 |||
   (bs.get ⟨offset + 5, by omega⟩).toUInt64 <<< 0x28 |||
@@ -32,21 +57,44 @@ def ByteArray.getUInt64LEfrom (bs : ByteArray) (offset : Nat) (h: bs.size - offs
   (bs.get ⟨offset + 1, by omega⟩).toUInt64 <<< 0x08 |||
   (bs.get ⟨offset + 0, by omega⟩).toUInt64
 
-def ByteArray.getUInt32LEfrom (bs : ByteArray) (offset : Nat) (h: bs.size - offset ≥ 4) : UInt32 := 
+def UInt64.getBytesLEfrom (i : UInt64) : ByteArray :=
+  ⟨#[ (i >>> 0x00).toUInt8
+    , (i >>> 0x8).toUInt8
+    , (i >>> 0x10).toUInt8
+    , (i >>> 0x18).toUInt8
+    , (i >>> 0x20).toUInt8
+    , (i >>> 0x28).toUInt8
+    , (i >>> 0x30).toUInt8
+    , (i >>> 0x38).toUInt8
+    ]⟩
+
+def ByteArray.getUInt32LEfrom (bs : ByteArray) (offset : Nat) (h: bs.size - offset ≥ 4) : UInt32 :=
   (bs.get ⟨offset + 3, by omega⟩).toUInt32 <<< 0x18 |||
   (bs.get ⟨offset + 2, by omega⟩).toUInt32 <<< 0x10 |||
   (bs.get ⟨offset + 1, by omega⟩).toUInt32 <<< 0x08 |||
   (bs.get ⟨offset + 0, by omega⟩).toUInt32
 
-def ByteArray.getUInt16LEfrom (bs : ByteArray) (offset : Nat) (h: bs.size - offset ≥ 2) : UInt16 := 
+def UInt32.getBytesLEfrom (i : UInt32) : ByteArray :=
+  ⟨#[ (i >>> 0x00).toUInt8
+    , (i >>> 0x8).toUInt8
+    , (i >>> 0x10).toUInt8
+    , (i >>> 0x18).toUInt8
+    ]⟩
+
+def ByteArray.getUInt16LEfrom (bs : ByteArray) (offset : Nat) (h: bs.size - offset ≥ 2) : UInt16 :=
   (bs.get ⟨offset + 1, by omega⟩).toUInt16 <<< 0x08 |||
   (bs.get ⟨offset + 0, by omega⟩).toUInt16
+
+def UInt16.getBytesLEfrom (i : UInt16) : ByteArray :=
+  ⟨#[ (i >>> 0x00).toUInt8
+    , (i >>> 0x8).toUInt8
+    ]⟩
 
 /- An alternative approach is to define a byte parsing monad, à la:
 
 https://github.com/risc0/risc0-lean4/blob/31c956fc9246bbfc84359021d66ed94972afd86b/R0sy/ByteDeserial.lean
 
-And just have some runtime error possibilities, rather than proof obligations. 
+And just have some runtime error possibilities, rather than proof obligations.
 -/
 
 def ByteArray.getEntriesFrom
@@ -59,7 +107,7 @@ def ByteArray.getEntriesFrom
   (spaceAvail : bs.size ≥ offset + num * entsize)
   (toEnt :  (offset₂ : Nat) → (bs.size - offset₂ ≥ entreq) → α)
   : List α := recur num [] (by omega)
-  where recur (idx : Nat) acc (h₁ : idx ≤ num) : List α 
+  where recur (idx : Nat) acc (h₁ : idx ≤ num) : List α
   := match idx with
     | 0 => acc
     | i + 1 =>
@@ -77,18 +125,18 @@ structure NByteArray (n : Nat) where
   sized: bytes.size = n
 
 instance : Repr (NByteArray n) where
-  reprPrec nbs := reprPrec $ nbs.bytes.toList.map λbyte ↦ 
-    Nat.toDigits 16 byte.toNat 
-    |> (λl ↦ if l.length == 1 then '0' :: l else l) 
+  reprPrec nbs := reprPrec $ nbs.bytes.toList.map λbyte ↦
+    Nat.toDigits 16 byte.toNat
+    |> (λl ↦ if l.length == 1 then '0' :: l else l)
     |> List.asString
 
 instance : Repr ByteArray where
-  reprPrec nbs := reprPrec $ nbs.data.toList.map λbyte ↦ 
-    Nat.toDigits 16 byte.toNat 
-    |> (λl ↦ if l.length == 1 then '0' :: l else l) 
+  reprPrec nbs := reprPrec $ nbs.data.toList.map λbyte ↦
+    Nat.toDigits 16 byte.toNat
+    |> (λl ↦ if l.length == 1 then '0' :: l else l)
     |> List.asString
 
-/- 
+/-
 
  These are some simple theorems related to Arrays and ByteArrays. They start
  from the function Array.extract.loop, associated with Array.extract:
@@ -111,7 +159,7 @@ instance : Repr ByteArray where
  ∀{a: ByteArray}, ByteArray.empty ++ a = a
 
  It would also be good to improve NByteArray extract to take an offset in addition to a length
--/ 
+-/
 
 theorem Array.extract_len_aux {src: Array α} :
    ∀b l dst, (b + l ≤ src.size) →
@@ -119,7 +167,7 @@ theorem Array.extract_len_aux {src: Array α} :
    intro b
    induction b
    case zero => simp [Array.extract.loop]
-   case succ => 
+   case succ =>
      rename_i n ih
      intro l dst
      unfold Array.extract.loop
@@ -148,7 +196,7 @@ def NByteArray.extract (bs : ByteArray) (n : Nat) (h : bs.size ≥ n) : NByteArr
            , ByteArray.empty
            , ByteArray.mkEmpty
            ]
-      have : ∀α, ∀n : Nat, @Array.extract.loop α #[] 0 n #[] = #[] := by 
+      have : ∀α, ∀n : Nat, @Array.extract.loop α #[] 0 n #[] = #[] := by
         unfold Array.extract.loop
         split; simp; contradiction
       rw [this, this]
@@ -166,3 +214,102 @@ def NByteArray.extract (bs : ByteArray) (n : Nat) (h : bs.size ≥ n) : NByteArr
         · assumption
         · simp [Nat.min_def, ByteArray.size, Array.size] at *
     ⟨bytes, proof⟩
+
+theorem UInt16.ByteArray_size : ∀ i : UInt16, i.getBytesBEfrom.size = 2 := by
+  intro i
+  simp [UInt16.getBytesBEfrom, ByteArray.size]
+
+theorem UInt16.eq_of_val_eq : ∀{i j : UInt16}, i.val = j.val → i = j
+  | ⟨_, _⟩, ⟨_, _⟩, rfl => rfl
+
+theorem UInt8.eq_of_val_eq : ∀{i j : UInt8}, i.val = j.val → i = j
+  | ⟨_, _⟩, ⟨_, _⟩, rfl => rfl
+
+theorem UInt8_to_UInt16_round: ∀{i : UInt8}, i.toUInt16.toUInt8 = i := by
+  intro i
+  cases i
+  rename_i i
+  simp [UInt16.toUInt8, Nat.toUInt8, UInt8.ofNat]
+  apply UInt8.eq_of_val_eq
+  simp
+  cases i
+  rename_i val lt
+  apply Fin.eq_of_val_eq
+  simp [Fin.ofNat, UInt16.toNat, UInt8.toUInt16, Nat.toUInt16, UInt16.ofNat, UInt8.toNat]
+  unfold UInt8.size at lt
+  simp_arith
+  apply Nat.mod_eq_of_lt
+  exact lt
+
+theorem UInt16_to_UInt8_round: ∀{i : UInt16}, i.toUInt8.toUInt16 = i % 256:= by
+  intro i
+  cases i
+  rename_i i
+  simp [UInt8.toUInt16, Nat.toUInt16, UInt16.ofNat]
+  unfold HMod.hMod
+  simp [instHMod, Mod.mod, UInt16.mod]
+  apply UInt16.eq_of_val_eq
+  simp [Fin.ofNat, UInt8.toNat, UInt16.toUInt8, Nat.toUInt8, UInt8.ofNat, UInt8.toNat, UInt16.toNat, Fin.mod]
+  apply Nat.mod_eq_of_lt
+  have : ↑i % 256 < 256 := @Nat.mod_lt ↑i 256 (by omega)
+  omega
+
+theorem Nat.bitwise_sum : ∀n m k : Nat, m % 2^n = 0 → k < 2^n → Nat.bitwise or m k = m + k := by
+  intro n
+  induction n
+  case zero =>
+    intro m k _ h₂
+    simp_arith at *
+    rw [h₂]
+    simp [Nat.bitwise]
+    intro h₃
+    apply Eq.symm
+    assumption
+  case succ n ih =>
+    intro m k h₁ h₂
+    have l₀ := (Nat.dvd_iff_mod_eq_zero (2 ^ Nat.succ n) m).mpr h₁
+    have l₁ : Dvd.dvd 2 m := by
+      refine Nat.dvd_of_pow_dvd ?_ l₀
+      simp_arith
+    have l₂ : m % 2 = 0 := by
+      apply Nat.mod_eq_zero_of_dvd
+      assumption
+    have l₃ : (m / 2) % 2 ^ n = 0 := by
+      apply (Nat.dvd_iff_mod_eq_zero (2 ^ n) (m / 2)).mp
+      apply Nat.dvd_of_mul_dvd_mul_right (k := 2) (by decide)
+      rw [Nat.div_mul_cancel l₁]
+      rw [←Nat.pow_succ]
+      assumption
+    have l₄ : (k /2) < 2 ^ n := by
+      simp [Nat.pow_succ] at h₂
+      apply Nat.div_lt_of_lt_mul
+      rw [Nat.mul_comm]
+      assumption
+    unfold Nat.bitwise
+    split <;> simp_arith
+    . apply Eq.symm; assumption
+    . split
+      . simp_arith; apply Eq.symm; assumption
+      . split
+        case inr.inr.inl h₃ h₄ h₅ =>
+          cases h₅
+          case inl h₅ => rw [l₂] at h₅; contradiction
+          case inr h₅ =>
+            have ih := ih (m/2) (k/2) l₃ l₄
+            simp_arith [ih]
+            rw [Nat.mul_comm, Nat.div_mul_cancel l₁]
+            simp_arith
+            conv =>
+              rhs
+              rw [←Nat.mod_add_div k 2]
+            simp_arith [h₅]
+        case inr.inr.inr h₃ h₄ h₅ =>
+            have ih := ih (m/2) (k/2) l₃ l₄
+            rw [ih]
+            simp_arith
+            rw [Nat.mul_comm, Nat.div_mul_cancel l₁]
+            cases (Nat.mod_two_eq_zero_or_one k)
+            case inr rhs => have c : m % 2 = 1 ∨ k % 2 = 1 := Or.inr rhs; contradiction
+            case inl lhs =>
+              have : Dvd.dvd 2 k := (Nat.dvd_iff_mod_eq_zero 2 k).mpr lhs
+              rw [Nat.mul_comm, Nat.div_mul_cancel this]
